wip

Foundation/Modal/Kripke/Logic/K4McK.lean
@@ -17,29 +17,29 @@ abbrev FrameClass.K4McK : FrameClass := { F | F.IsK4McK }
 end Kripke
 
 
-namespace Logic.K4McK.Kripke
+namespace Hilbert.K4McK.Kripke
 
-instance sound : Sound Logic.K4McK FrameClass.K4McK := instSound_of_validates_axioms $ by
+instance : Sound Hilbert.K4McK FrameClass.K4McK := instSound_of_validates_axioms $ by
   apply FrameClass.Validates.withAxiomK;
   rintro F ⟨_, _⟩ _ (rfl | rfl);
   . exact validate_AxiomFour_of_transitive;
   . exact validate_axiomMcK_of_satisfiesMcKinseyCondition;
 
-instance consistent : Entailment.Consistent Logic.K4McK := consistent_of_sound_frameclass FrameClass.K4McK $ by
+instance : Entailment.Consistent Hilbert.K4McK := consistent_of_sound_frameclass FrameClass.K4McK $ by
   use whitepoint;
   constructor;
 
-instance canonical : Canonical Logic.K4McK FrameClass.K4McK := ⟨by constructor⟩
+instance : Canonical Hilbert.K4McK FrameClass.K4McK := ⟨by constructor⟩
 
-instance complete : Complete Logic.K4McK FrameClass.K4McK := inferInstance
+instance : Complete Hilbert.K4McK FrameClass.K4McK := inferInstance
 
-lemma trans_mckinsey : Logic.K4McK = FrameClass.K4McK.logic := eq_hilbert_logic_frameClass_logic
+lemma trans_mckinsey : Modal.K4McK = FrameClass.K4McK.logic := eq_hilbert_logic_frameClass_logic
 
-instance : Logic.K4 ⪱ Logic.K4McK := by
+instance : Hilbert.K4 ⪱ Hilbert.K4McK := by
   constructor;
   . apply Hilbert.weakerThan_of_subset_axioms; simp;
   . apply Entailment.not_weakerThan_iff.mpr;
-    suffices ∃ φ, Logic.K4McK ⊢! φ ∧ ¬FrameClass.K4 ⊧ φ by simpa [K4.Kripke.trans];
+    suffices ∃ φ, Hilbert.K4McK ⊢! φ ∧ ¬FrameClass.K4 ⊧ φ by simpa [K4.Kripke.trans];
     use (Axioms.McK (.atom 0));
     constructor;
     . exact axiomMcK!;
@@ -49,6 +49,8 @@ instance : Logic.K4 ⪱ Logic.K4McK := by
       . simp only [Set.mem_setOf_eq]; refine { trans := by simp; }
       . simp [Semantics.Realize, Satisfies];
 
-end Logic.K4McK.Kripke
+end Hilbert.K4McK.Kripke
+
+instance : Modal.K4 ⪱ Modal.K4McK := inferInstance
 
 end LO.Modal
