Foundation/Modal/Kripke/Logic/K4Point3.lean
@@ -22,32 +22,32 @@ end Kripke
 
 namespace Logic.K4Point3.Kripke
 
-instance sound : Sound Logic.K4Point3 FrameClass.IsK4Point3 := instSound_of_validates_axioms $ by
+instance : Sound Hilbert.K4Point3 FrameClass.IsK4Point3 := instSound_of_validates_axioms $ by
   apply FrameClass.Validates.withAxiomK;
   rintro F ⟨_, _⟩ _ (rfl | rfl);
   . exact validate_AxiomFour_of_transitive;
   . exact validate_WeakPoint3_of_weakConnected;
 
-instance consistent : Entailment.Consistent Logic.K4Point3 :=
+instance : Entailment.Consistent Hilbert.K4Point3 :=
   consistent_of_sound_frameclass FrameClass.IsK4Point3 $ by
     use whitepoint;
     constructor;
 
-instance canonical : Canonical Logic.K4Point3 FrameClass.IsK4Point3 :=  ⟨by constructor⟩
+instance : Canonical Hilbert.K4Point3 FrameClass.IsK4Point3 :=  ⟨by constructor⟩
 
-instance complete : Complete Logic.K4Point3 FrameClass.IsK4Point3 := inferInstance
+instance : Complete Hilbert.K4Point3 FrameClass.IsK4Point3 := inferInstance
 
-lemma trans_weakConnected : Logic.K4Point3 = FrameClass.IsK4Point3.logic := eq_hilbert_logic_frameClass_logic
+lemma trans_weakConnected : Modal.K4Point3 = FrameClass.IsK4Point3.logic := eq_hilbert_logic_frameClass_logic
 
-instance : Logic.K4 ⪱ Logic.K4Point3 := by
+instance : Hilbert.K4 ⪱ Hilbert.K4Point3 := by
   constructor;
-  . apply Hilbert.weakerThan_of_subset_axioms $ by simp;
+  . apply Hilbert.Normal.weakerThan_of_subset_axioms $ by simp;
   . apply Entailment.not_weakerThan_iff.mpr;
-    suffices ∃ φ, Logic.K4Point3 ⊢! φ ∧ ¬FrameClass.K4 ⊧ φ by simpa [K4.Kripke.trans];
     use (Axioms.WeakPoint3 (.atom 0) (.atom 1));
     constructor;
     . exact axiomWeakPoint3!;
-    . apply Kripke.not_validOnFrameClass_of_exists_model_world;
+    . apply Sound.not_provable_of_countermodel (𝓜 := FrameClass.K4)
+      apply Kripke.not_validOnFrameClass_of_exists_model_world;
       let M : Model := ⟨
         ⟨Fin 3, λ x y => x = 0 ∧ y ≠ 0⟩,
         λ w a => if a = 0 then w = 1 else w = 2
