Foundation/Modal/Kripke/Logic/KDB.lean
@@ -20,34 +20,34 @@ abbrev FrameClass.KDB : FrameClass := { F | F.IsKDB }
 end Kripke
 
 
-namespace Logic.KDB.Kripke
+namespace Hilbert.KDB.Kripke
 
-instance sound : Sound (Hilbert.KDB) Kripke.FrameClass.KDB := instSound_of_validates_axioms $ by
+instance : Sound (Hilbert.KDB) Kripke.FrameClass.KDB := instSound_of_validates_axioms $ by
   apply FrameClass.Validates.withAxiomK;
   rintro F ⟨_, _⟩ _ (rfl | rfl);
   . exact validate_AxiomD_of_serial;
   . exact validate_AxiomB_of_symmetric;
 
-instance consistent : Entailment.Consistent (Hilbert.KDB) := consistent_of_sound_frameclass Kripke.FrameClass.KDB $ by
+instance : Entailment.Consistent (Hilbert.KDB) := consistent_of_sound_frameclass Kripke.FrameClass.KDB $ by
   use whitepoint;
   constructor;
 
 
-instance canonical : Canonical (Hilbert.KDB) Kripke.FrameClass.KDB := ⟨by constructor⟩
+instance : Canonical (Hilbert.KDB) Kripke.FrameClass.KDB := ⟨by constructor⟩
 
-instance complete : Complete (Hilbert.KDB) Kripke.FrameClass.KDB := inferInstance
+instance : Complete (Hilbert.KDB) Kripke.FrameClass.KDB := inferInstance
 
-lemma serial_symm : Logic.KDB = Kripke.FrameClass.KDB.logic := eq_hilbert_logic_frameClass_logic
+lemma serial_symm : Modal.KDB = Kripke.FrameClass.KDB.logic := eq_hilbert_logic_frameClass_logic
 
-instance : Logic.KD ⪱ Logic.KDB := by
+instance : Hilbert.KD ⪱ Hilbert.KDB := by
   constructor;
-  . apply Hilbert.weakerThan_of_subset_axioms $ by simp;
+  . apply Hilbert.Normal.weakerThan_of_subset_axioms $ by simp;
   . apply Entailment.not_weakerThan_iff.mpr;
-    suffices ∃ φ, Logic.KDB ⊢! φ ∧ ¬FrameClass.IsKD ⊧ φ by simpa [KD.Kripke.serial];
     use Axioms.B (.atom 0);
     constructor;
     . exact axiomB!;
-    . apply Kripke.not_validOnFrameClass_of_exists_model_world;
+    . apply Sound.not_provable_of_countermodel (𝓜 := FrameClass.IsKD)
+      apply Kripke.not_validOnFrameClass_of_exists_model_world;
       let M : Model := ⟨⟨Fin 2, λ x y => x ≤ y⟩, λ w _ => w = 0⟩;
       use M, 0;
       constructor;
@@ -56,20 +56,20 @@ instance : Logic.KD ⪱ Logic.KDB := by
         use 1;
         constructor <;> omega;
 
-instance : Logic.KB ⪱ Logic.KDB := by
+instance : Hilbert.KB ⪱ Hilbert.KDB := by
   constructor;
-  . apply Hilbert.weakerThan_of_subset_axioms $ by simp;
+  . apply Hilbert.Normal.weakerThan_of_subset_axioms $ by simp;
   . apply Entailment.not_weakerThan_iff.mpr;
-    suffices ∃ φ, Logic.KDB ⊢! φ ∧ ¬FrameClass.KB ⊧ φ by simpa [KB.Kripke.symm];
     use Axioms.D (.atom 0);
     constructor;
     . exact axiomD!;
-    . apply Kripke.not_validOnFrameClass_of_exists_model_world;
+    . apply Sound.not_provable_of_countermodel (𝓜 := FrameClass.KB)
+      apply Kripke.not_validOnFrameClass_of_exists_model_world;
       use ⟨⟨Fin 1, λ x y => False⟩, λ w _ => w = 0⟩, 0;
       constructor;
       . refine { symm := by simp; };
       . simp [Semantics.Realize, Satisfies];
 
-end Logic.KDB.Kripke
+end Hilbert.KDB.Kripke
 
 end LO.Modal
