Foundation/Modal/Kripke/Logic/S4.lean
@@ -21,26 +21,26 @@ protected abbrev FrameClass.finite_S4 : FrameClass := { F | F.IsFiniteS4 }
 end Kripke
 
 
-namespace Logic.S4.Kripke
+namespace Hilbert.S4.Kripke
 
-instance sound : Sound Logic.S4 FrameClass.S4 := instSound_of_validates_axioms $ by
+instance : Sound Hilbert.S4 FrameClass.S4 := instSound_of_validates_axioms $ by
   apply FrameClass.Validates.withAxiomK;
   rintro F ⟨_, _⟩ _ (rfl | rfl);
   . exact validate_AxiomT_of_reflexive;
   . exact validate_AxiomFour_of_transitive;
 
-instance consistent : Entailment.Consistent Logic.S4 := consistent_of_sound_frameclass FrameClass.S4 $ by
+instance : Entailment.Consistent Hilbert.S4 := consistent_of_sound_frameclass FrameClass.S4 $ by
   use whitepoint;
   constructor;
 
-instance canonical : Canonical Logic.S4 FrameClass.S4 := ⟨by constructor⟩
+instance : Canonical Hilbert.S4 FrameClass.S4 := ⟨by constructor⟩
 
-instance complete : Complete Logic.S4 FrameClass.S4 := inferInstance
+instance : Complete Hilbert.S4 FrameClass.S4 := inferInstance
 
 open finestFiltrationTransitiveClosureModel in
-instance finiteComplete : Complete Logic.S4 FrameClass.finite_S4 := ⟨by
+instance : Complete Hilbert.S4 FrameClass.finite_S4 := ⟨by
   intro φ hp;
-  apply Kripke.complete.complete;
+  apply Complete.complete (𝓜 := FrameClass.S4);
   rintro F hF V x;
   replace hF := Set.mem_setOf_eq.mp hF;
   let M : Kripke.Model := ⟨F, V⟩;
@@ -53,17 +53,17 @@ instance finiteComplete : Complete Logic.S4 FrameClass.finite_S4 := ⟨by
   }
 ⟩
 
-lemma preorder : Logic.S4 = FrameClass.S4.logic := eq_hilbert_logic_frameClass_logic
+lemma preorder : Modal.S4 = FrameClass.S4.logic := eq_hilbert_logic_frameClass_logic
 
-instance : Logic.KT ⪱ Logic.S4 := by
+instance : Hilbert.KT ⪱ Hilbert.S4 := by
   constructor;
-  . apply Hilbert.weakerThan_of_subset_axioms $ by simp;
+  . apply Hilbert.Normal.weakerThan_of_subset_axioms $ by simp;
   . apply Entailment.not_weakerThan_iff.mpr;
-    suffices ∃ φ, Logic.S4 ⊢! φ ∧ ¬FrameClass.KT ⊧ φ by simpa [KT.Kripke.refl];
     use Axioms.Four (.atom 0);
     constructor;
     . exact axiomFour!;
-    . apply Kripke.not_validOnFrameClass_of_exists_model_world;
+    . apply Sound.not_provable_of_countermodel (𝓜 := FrameClass.KT)
+      apply Kripke.not_validOnFrameClass_of_exists_model_world;
       let M : Model := ⟨
           ⟨Fin 3, λ x y => (x = 0 ∧ y ≠ 2) ∨ (x = 1 ∧ y ≠ 0) ∨ (x = 2 ∧ y = 2)⟩,
           λ w _ => w = 0 ∨ w = 1
@@ -85,16 +85,16 @@ instance : Logic.KT ⪱ Logic.S4 := by
           . use 2;
             refine ⟨by omega;, by trivial, by trivial⟩;
 
-instance : Logic.KD4 ⪱ Logic.S4 := by
+instance : Hilbert.KD4 ⪱ Hilbert.S4 := by
   constructor;
-  . apply Hilbert.weakerThan_of_provable_axioms;
+  . apply Hilbert.Normal.weakerThan_of_provable_axioms;
     rintro _ (rfl | rfl | rfl) <;> simp
   . apply Entailment.not_weakerThan_iff.mpr;
-    suffices ∃ φ, Logic.S4 ⊢! φ ∧ ¬FrameClass.KD4 ⊧ φ by simpa [KD4.Kripke.serial_trans];
     use Axioms.T (.atom 0);
     constructor;
     . exact axiomT!;
-    . apply Kripke.not_validOnFrameClass_of_exists_model_world;
+    . apply Sound.not_provable_of_countermodel (𝓜 := FrameClass.KD4)
+      apply Kripke.not_validOnFrameClass_of_exists_model_world;
       use ⟨⟨Fin 3, λ _ y => y = 1⟩, (λ w _ => w = 1)⟩, 0;
       constructor;
       . refine {
@@ -103,10 +103,16 @@ instance : Logic.KD4 ⪱ Logic.S4 := by
         };
       . simp [Semantics.Realize, Satisfies];
 
-instance : Logic.KD ⪱ Logic.S4 := calc
-  Logic.KD ⪱ Logic.KD4 := by infer_instance
-  _        ⪱ Logic.S4  := by infer_instance
+instance : Hilbert.KD ⪱ Hilbert.S4 := calc
+  Hilbert.KD ⪱ Hilbert.KD4 := by infer_instance
+  _          ⪱ Hilbert.S4  := by infer_instance
 
-end Logic.S4.Kripke
+end Hilbert.S4.Kripke
+
+instance : Modal.KT ⪱ Modal.S4 := inferInstance
+
+instance : Modal.KD4 ⪱ Modal.S4 := inferInstance
+
+instance : Modal.KD ⪱ Modal.S4 := inferInstance
 
 end LO.Modal
