Foundation/Modal/Kripke/Logic/S4McK.lean
@@ -22,31 +22,31 @@ end Kripke
 
 
 
-namespace Logic.S4McK.Kripke
+namespace Hilbert.S4McK.Kripke
 
-instance sound : Sound Logic.S4McK FrameClass.S4McK := instSound_of_validates_axioms $ by
+instance : Sound Hilbert.S4McK FrameClass.S4McK := instSound_of_validates_axioms $ by
   apply FrameClass.Validates.withAxiomK;
   rintro F ⟨_, _⟩ _ (rfl | rfl | rfl);
   . exact validate_AxiomT_of_reflexive;
   . exact validate_AxiomFour_of_transitive;
   . exact validate_axiomMcK_of_satisfiesMcKinseyCondition;
 
-instance consistent : Entailment.Consistent Logic.S4McK := consistent_of_sound_frameclass FrameClass.S4McK $ by
+instance : Entailment.Consistent Hilbert.S4McK := consistent_of_sound_frameclass FrameClass.S4McK $ by
   use whitepoint;
   apply Set.mem_setOf_eq.mpr;
   constructor
 
-instance canonical : Canonical Logic.S4McK FrameClass.S4McK := ⟨by constructor⟩
+instance : Canonical Hilbert.S4McK FrameClass.S4McK := ⟨by constructor⟩
 
-instance complete : Complete Logic.S4McK FrameClass.S4McK := inferInstance
+instance : Complete Hilbert.S4McK FrameClass.S4McK := inferInstance
 
-lemma preorder_mckinsey : Logic.S4McK = FrameClass.S4McK.logic := eq_hilbert_logic_frameClass_logic
+lemma preorder_mckinsey : Modal.S4McK = FrameClass.S4McK.logic := eq_hilbert_logic_frameClass_logic
 
-instance : Logic.S4 ⪱ Logic.S4McK := by
+instance : Hilbert.S4 ⪱ Hilbert.S4McK := by
   constructor;
   . apply Hilbert.weakerThan_of_subset_axioms; simp;
   . apply Entailment.not_weakerThan_iff.mpr;
-    suffices ∃ φ, Logic.S4McK ⊢! φ ∧ ¬FrameClass.S4 ⊧ φ by simpa [S4.Kripke.preorder];
+    suffices ∃ φ, Hilbert.S4McK ⊢! φ ∧ ¬FrameClass.S4 ⊧ φ by simpa [S4.Kripke.preorder];
     use (Axioms.McK (.atom 0));
     constructor;
     . exact axiomMcK!;
@@ -62,11 +62,11 @@ instance : Logic.S4 ⪱ Logic.S4McK := by
         use 1;
         trivial;
 
-instance : Logic.K4McK ⪱ Logic.S4McK := by
+instance : Hilbert.K4McK ⪱ Hilbert.S4McK := by
   constructor;
   . apply Hilbert.weakerThan_of_subset_axioms; intro φ; aesop;
   . apply Entailment.not_weakerThan_iff.mpr;
-    suffices ∃ φ, Logic.S4McK ⊢! φ ∧ ¬FrameClass.K4McK ⊧ φ by simpa [K4McK.Kripke.trans_mckinsey];
+    suffices ∃ φ, Hilbert.S4McK ⊢! φ ∧ ¬FrameClass.K4McK ⊧ φ by simpa [K4McK.Kripke.trans_mckinsey];
     use (Axioms.T (.atom 0));
     constructor;
     . simp;
@@ -83,6 +83,10 @@ instance : Logic.K4McK ⪱ Logic.S4McK := by
         }
       . simp [Semantics.Realize, Satisfies, M];
 
-end Logic.S4McK.Kripke
+end Hilbert.S4McK.Kripke
+
+instance : Modal.S4 ⪱ Modal.S4McK := inferInstance
+
+instance : Modal.K4McK ⪱ Modal.S4McK := inferInstance
 
 end LO.Modal
